update

Test.lean
@@ -1,144 +1,1517 @@
-import Mathlib.Tactic.Basic
-import Mathlib.Tactic.LeftRight
+import Theory
+import Lean.Data.PersistentHashMap
+
+open Lean PersistentHashMap
 
 
-lemma v1 (P Q R : Prop) : P ∧ (Q ∨ R) ↔ (P ∧ Q) ∨ (P ∧ R) := by
-(constructor;
-  (intro h;
-    cases h with 
-      | intro hP hQR =>
-        cases hQR with
-          | inl hQ => 
-            left; constructor;
-              assumption;
-              assumption
-          | inr hR => 
-            right; constructor;
-                assumption;
-              assumption
-  );
-  (intro h;
-    cases h with
-      | inl hPQ => 
-        cases hPQ with 
-          | intro hP hQ => 
-            constructor;
-              assumption;
-              left; assumption
-      | inr hPR =>
-        cases hPR with
-          | intro hP hR =>
-            constructor;
-              assumption;
-              right; assumption
+#eval [: β[0] :]
+#eval [: β[0] :]
+
+#check [: β[0] ∨ α[0] :]
+#check [: β[0] ∧ α[0] :]
+#check [: β[0] × α[0] :]
+#check [: β[0] + α[0] :]
+def x := 0
+#check [: ∀ 1 :: β[0] ≤ α[0] => β[⟨x⟩] :]
+#check [: ∀ 1 :: β[0] ≤ α[0] => β[0] :]
+#check [: ∀ 2 :: α[0] ≤ α[0] => β[0] :]
+#check [: ∀ 2 => β[0] :]
+#check [: @ :]
+#check [: α[24] :]
+#check [: foo * @ :]
+#check [: foo * @ ∨ (boo * @) :]
+#check [: μ β[0] => foo * @ :]
+#check [: foo * boo * @ :]
+#check [: μ β[0] => foo * boo * @ :]
+#check [: μ β[0] => foo * β[0] :]
+#check [: μ β[0] => foo * β[0] ∧ α[0] ∨ α[2] ∧ α[0]:]
+#check [: β[3] ∧ α[0] -> α[1] ∨ α[2] :]
+#check [: μ β[0] => foo * β[0] ∧ α[0] ∨ α[2] ∧ α[0] -> α[1] ∨ α[2] :]
+#check [: μ β[0] => foo * β[0] ∧ α[0] ∨ α[2] ∧ α[0] :]
+#check [: α[0] :]
+
+#eval [: ∀ 2 :: α[0] ≤ α[0] => β[0] :]
+#eval [: μ β[0] => foo * β[0] ∧ α[0] ∨ α[2] ∧ α[0] :]
+
+
+#eval ({} : PHashMap Nat Ty)
+
+def zero_ := [: 
+    zero * @
+:]
+
+#eval unify_test [:
+    (dumb*@)
+:] zero_
+
+#eval unify_test [:
+    (zero*@)
+:] zero_
+
+/-
+  μ nat .
+    zero*@ | 
+    succ*nat 
+-/
+def nat_ := [: 
+  μ β[0] => 
+    zero*@ ∨ 
+    succ*β[0]
+:]
+#eval nat_
+
+def even := [: 
+  μ β[0] => 
+    zero*@ ∨ 
+    succ*succ*β[0]
+:]
+
+
+def weven := [: 
+  μ β[0] => 
+    zero*@ ∨ 
+    succ*dumb*β[0]
+:]
+
+#eval unify_test weven nat_ 
+#eval unify_test even nat_ 
+#eval unify_test nat_ even
+
+
+#eval unify_test
+[: ∃ 2 :: β[0] ≤ ⟨even⟩ => β[0] × β[1]:] 
+[: ∃ 2 :: β[0] ≤ ⟨nat_⟩ => β[0] × β[1]:] 
+
+#eval unify_test 
+[: ∃ 2 :: ⟨even⟩ ≤ β[0] => β[0] × β[1]:] 
+[: ∃ 2 :: ⟨nat_⟩ ≤ β[0] => β[0] × β[1]:] 
+
+#eval unify_test 
+[: ∃ 2 :: β[0] ≤ ⟨nat_⟩ => β[0] × β[1]:] 
+[: ∃ 2 :: β[0] ≤ ⟨even⟩ => β[0] × β[1]:] 
+
+#eval unify_test 
+[: ∃ 2 :: ⟨nat_⟩ ≤ β[0] => β[0] × β[1]:] 
+[: ∃ 2 :: ⟨even⟩ ≤ β[0] => β[0] × β[1]:] 
+
+#eval unify_test 
+[: (zero*@) :] nat_ 
+
+#eval unify_test 
+[: (succ*(zero*@)) :] nat_ 
+
+#eval unify_test 
+[: (succ*(α[0])) :] 
+nat_ 
+
+#eval unify_reduce 
+[: (succ*(α[0])) :] 
+nat_ 
+[: α[0] :]
+
+def nat_list := [: 
+  μ β[0] => (
+    (l ~ zero*@ ∧ r ~ nil*@) ∨ 
+    (∃ 2 :: l ~ β[0] ∧ r ~ β[1] ≤ β[2] => 
+      (l ~ succ*β[0] ∧ r ~ cons*β[1]))
   )
+:]
+--  ∧ / ∧  
+def even_list := [: 
+  μ β[0] => (
+    (l ~ zero*@ ∧ r ~ nil*@) ∨ 
+    (∃ 2 :: l ~ β[0] ∧ r ~ β[1] ≤ β[2] => 
+      (l ~ succ*succ*β[0] ∧ r ~ cons*cons*β[1]))
+  )
+:]
+
+-- TODO
+#eval unify_test 
+  nat_list
+  even_list
+
+#eval unify_test 
+  even_list
+  nat_list
+
+#eval unify_test 
+[: ∃ 1 :: β[0] ≤ ⟨even⟩ => hello * β[0] :]
+[: ∃ 1 :: β[0] ≤ ⟨nat_⟩ => hello * β[0] :]
+
+#eval unify_test 
+[: ∃ 1 :: β[0] ≤ ⟨nat_⟩ => hello * β[0] :]
+[: ∃ 1 :: β[0] ≤ ⟨even⟩ => hello * β[0] :]
+
+#eval unify_test 
+  [: (l ~ zero*@ ∧ r ~ nil*@) :] 
+  nat_list
+
+#eval unify_test 
+  [: (l ~ zero*@ ∧ r ~ dumb*@) :] 
+  nat_list
+
+-- this is record type is not wellformed 
+#eval unify_test 
+  [: (l ~ α[0] ∧ r ~ α[1]) :] 
+  nat_list
+
+-- this is record type is not wellformed 
+#eval unify_reduce
+  [: (l ~ α[0] ∧ r ~ α[1]) :] 
+  nat_list
+  [: ⊤ :]
+
+#eval unify_test 
+  [: (l ~ zero*@ ∧ r ~ α[0]) :] 
+  nat_list
+
+-- expected α[0] → /nil
+#eval unify_test 
+  [: (l ~ succ*zero*@ ∧ r ~ cons*α[0]) :] 
+  nat_list
+
+#eval unify_test 
+  [: (l ~ succ*succ*zero*@ ∧ r ~ cons*α[0]) :] 
+  nat_list
+
+
+#eval unify_reduce 
+  [: (l ~ succ*succ*zero*@ ∧ r ~ cons*α[0]) :] 
+  nat_list
+  [: α[0]:]
+
+
+#eval unify_test 
+  [: (l ~ succ*zero*@ ∧ r ~ cons*cons*α[0]) :] 
+  nat_list
+
+
+
+def nat_to_list := [: 
+  ν β[0] => 
+    (zero*@ -> nil*@) ∧ 
+    (∀ 2 :: β[2] ≤ β[0] -> β[1] => 
+      succ*β[0] -> cons*β[1])
+:]
+
+#eval unify_test 
+  nat_to_list
+  [: (succ*zero*@) -> (cons*nil*@) :] 
+
+#eval unify_reduce 
+  nat_to_list
+  [: (succ*zero*@) -> (cons*nil*@) :] 
+  [: ⊤ :]
+
+#eval unify_reduce
+  nat_to_list
+  [: (succ*zero*@ -> cons*α[0]) :] 
+  [: α[0] :]
+
+#eval unify_reduce
+  nat_to_list
+  [: (succ*zero*@ -> cons*cons*α[0]) :] 
+  [: α[0] :]
+
+
+/-
+  μ plus .
+    ∃ N .  
+      zero*@ × N × N | 
+
+    ∃ X Y Z :: X, Y, Z ≤ plus .  
+      succ*X × Y × succ*Z
+-/
+def plus := [: 
+  μ β[0] => 
+    (∃ 1 => 
+      (x ~ zero*@ ∧ y ~ β[0] ∧ z ~ β[0])) ∨ 
+
+    (∃ 3 :: (x ~ β[0] ∧ y ~ β[1] ∧ z ~ β[2]) ≤ β[3] => 
+      (x ~ succ*β[0] ∧ y ~ β[1] ∧ z ~ succ*β[2]))
+:]
+
+-- /print plus
+
+-- #eval [: (x ~ zero*@ ∧ y ~ zero*@ ∧ z ~ zero*@) :]  
+-- #eval [: succ*succ*zero*@ :]  
+
+
+#eval unify_reduce [:
+    x ~ zero*@ ∧ 
+    y ~ α[0] ∧ 
+    z ~ zero*@
+:] plus [: α[0] :]
+
+
+#eval unify_reduce [:
+  (
+    x ~ (succ*zero*@) ∧ 
+    y ~ (succ*zero*@) ∧ 
+    z ~ (α[0])
+  )
+:] plus [: α[0] :]
+
+
+#eval unify_reduce [:
+  (
+    x ~ (succ*succ*zero*@) ∧ 
+    y ~ (succ*zero*@) ∧
+    z ~ (α[0])
+  )
+:] plus
+[: α[0] :]
+
+#eval unify_reduce [:
+  (
+    x ~ (succ*zero*@) ∧ 
+    y ~ (α[0]) ∧
+    z ~ (succ*succ*zero*@)
+  )
+:] plus
+[: α[0] :]
+
+#eval unify_reduce [:
+  (
+    x ~ (succ*zero*@) ∧
+    y ~ (succ*succ*zero*@) ∧
+    z ~ (α[0])
+  )
+:] plus [: α[0] :]
+
+
+-- expected: α[0] ↦ succ*zero*@
+#eval unify_reduce [:
+(
+  x ~ α[0] ∧
+  y ~ succ*zero*@ ∧
+  z ~ succ*succ*zero*@
 )
-
-lemma v2 (P Q R : Prop) : P ∧ (Q ∨ R) ↔ (P ∧ Q) ∨ (P ∧ R) := 
-  ((Iff.intro
-    ((λ h : P ∧ (Q ∨ R) =>
-      (match h with
-        | And.intro hP hQR => (match hQR with
-            | Or.inl hQ => Or.inl (And.intro hP hQ : P ∧ Q)
-            | Or.inr hR => Or.inr (And.intro hP hR : P ∧ R)
-        )
-      )
-    ) : P ∧ (Q ∨ R) -> (P ∧ Q) ∨ (P ∧ R))
-    ((λ h : P ∧ Q ∨ P ∧ R =>
-      (And.intro 
-        ((match h with
-          | Or.inl (And.intro hP hQ) => hP
-          | Or.inr (And.intro hP hR) => hP
-        ) : P)
-        ((match h with
-          | Or.inl (And.intro hP hQ) => Or.inl hQ 
-          | Or.inr (And.intro hP hR) => Or.inr hR
-        ) : Q ∨ R)
-      )
-    ) : (P ∧ Q) ∨ (P ∧ R) -> P ∧ (Q ∨ R))
-  ) : P ∧ (Q ∨ R) ↔ (P ∧ Q) ∨ (P ∧ R))
-
-class MyAdd (a : Type) where
-  add : a -> a -> a
-
-#check @MyAdd.add
-
-instance : MyAdd Nat where
-  add := Nat.add
-
-instance : MyAdd Int where
-  add := Int.add
-
-instance : MyAdd Float where
-  add := Float.add
-
-def double [inst : Add a] (x : a) : a :=
-  inst.add x x
-
-#check @double
--- @double : {a : Type} → [inst : Add a] → a → a
-
--- #eval double 10
--- 20
+:] plus
+[: α[0] :]
 
 
-
-#check Nat.ne_of_lt
-
-example : ¬ 0 < 0 :=
-  ((fun h => 
-    let x := (Nat.ne_of_lt h)
-    let y := (absurd rfl x)
-    y
-  ) : ¬ 0 < 0)
-
-#check @absurd
-example (n : Nat) (h : n ≠ 0) : .succ (.pred n) = n := 
-  ((match n with
-    | Nat.zero => absurd rfl h
-    | Nat.succ m => rfl 
-  ) : .succ (.pred n) = n)
-
-example (n : Nat) (h : n ≠ 0) : .succ (.pred n) = n := by
-  cases n with
-  | zero =>
-    -- goal: h : 0 ≠ 0 ⊢ succ (pred 0) = 0
-    apply absurd rfl h
-  | succ m =>
-    -- second goal: h : succ m ≠ 0 ⊢ succ (pred (succ m)) = succ m
-    rfl
+#eval unify_reduce [:
+(
+  x ~ succ*zero*@ ∧
+  y ~ α[0] ∧
+  z ~ succ*succ*zero*@
+)
+:] plus
+[: α[0] :]
 
 
--- induction with term and tactics
-def add : Nat → Nat → Nat
-  | m, .zero   => m
-  | m, .succ n => .succ (add m n)
+#eval unify_reduce [:
+(
+  x ~ (α[0]) ∧
+  y ~ (α[1]) ∧
+  z ~ (succ*succ*zero*@)
+)
+:] plus
+[: x ~ α[0] ∧ y ~ α[1] :]
 
-theorem add_zero (m : Nat)   : add m .zero = m := rfl
-theorem add_succ (m n : Nat) : add m (.succ n) = .succ (add m n) := rfl
+#eval unify_reduce [:
+(
+  x ~ (succ*succ*zero*@) ∧
+  y ~ (α[1]) ∧
+  z ~ (α[0])
+)
+:] plus
+[: y ~ α[1] ∧ z ~ α[0] :]
 
-theorem zero_add : ∀ n, add .zero n = n
-  | .zero   => rfl
-  | .succ n => congrArg Nat.succ (zero_add n)
 
-#check @congrArg
-example : ∀ n, add .zero n = n := by
-  (intro n;
-    (induction n with
-      | zero => apply rfl 
-      | succ n IH => apply congrArg Nat.succ IH
+-- term testing
+#eval [:
+  λ[ 
+    for y[0] : α[0] => y[0],
+    for y[0] : α[0] => y[0] 
+  ]
+:]
+
+#eval [:
+  ω[ 
+    left := x[0],
+    right := x[0]
+  ]
+:]
+
+
+#eval [:
+  succ;zero;()
+:]
+
+
+
+#eval infer_reduce [:
+  succ;zero;()
+:]
+
+#eval [:
+  succ;zero;()
+:]
+
+#eval [:
+  x[0]/hello
+:]
+
+#eval infer_reduce [:
+  _ 
+:]
+
+
+#eval [:
+  α[0] + α[1]
+:]
+
+#eval [:
+  α[0] × α[1]
+:]
+
+#eval [:
+  (x[0], x[1])
+:]
+
+
+#eval infer_reduce [:
+  λ [for y[0] => y[0]]
+:]
+
+#eval infer_reduce [:
+  λ [for y[0] : abc*@ => y[0]]
+:]
+
+#eval infer_reduce [:
+  λ [for y[0] : inp*@ -> out*@ =>
+  Out ; λ [for y[0] => 
+      cons ; ((y[1] y[0]), nil ; ())
+  ]
+  ]
+:]
+
+#eval infer_reduce [:
+  ((), nil ; ())
+:]
+
+  
+#eval [:
+  hello*thing~@
+  
+:]
+
+#eval infer_reduce [:
+  λ y[0] : nat*@ =>
+    let y[0] = (λ (y[0], y[1]) : (str*@ × str*@) => y[0]) =>
+    (y[0] (str;(), str;()))
+:]
+
+#eval infer_reduce [:
+  λ y[0] : nat*@ =>
+    let y[0] = (λ (y[0], y[1]) : (str*@ × str*@) => y[0]) =>
+    (y[0] (_, str;()))
+:]
+
+#eval infer_reduce [:
+  λ y[0] : nat*@ =>
+    let y[0] = λ[for (y[0], y[1]) : (str*@ × str*@) => y[0]] =>
+    (y[0] (y[1], _))
+:]
+
+-- Propagation: Down 
+-- even though, there is a hole in the program,
+-- the type of α[0] can be inferred to be uno*@  
+-- due to the application and downward propagation
+#eval infer_reduce [:
+  λ y[0] : α[0] =>
+    let y[0] = (λ (y[0], y[1]) : (uno*@ × dos*@) => y[1]) =>
+    (y[0] (y[1], _))
+:]
+
+-- Propagation: Up
+#eval infer_reduce [:
+  λ y[0] : hello*@ -> world*@ =>
+  λ y[0] => 
+    (cons ; ((y[1] y[0]), nil ; ()))
+:]
+
+#eval infer_reduce [:
+  λ y[0] : int*@ -> str*@ => 
+  λ y[0] : int*@  =>
+    (y[1] y[0])
+:]
+
+
+#eval infer_reduce [:
+  λ y[0] : str*@ -> @ => 
+  λ y[0] : str*@ => 
+     (OUTPUT ; (y[1] y[0]))
+:]
+
+#eval infer_reduce [:
+  λ y[0] : int*@ -> @ => 
+  λ y[0] : str*@ => 
+     (y[1] y[0]) 
+:]
+
+#eval infer_reduce [:
+  λ y[0] : (int*@ ∨ str*@) -> @ => 
+  λ y[0] : str*@ => 
+     (y[1] y[0]) 
+:]
+
+#eval infer_reduce [:
+  λ y[0] : (int*@ ∨ α[1]) -> α[1] => 
+  λ y[0] : str*@ => 
+     (y[1] y[0]) 
+:]
+
+#eval infer_reduce [:
+  λ y[0] : ∀ 1 => (β[0] -> β[0]) => 
+  λ y[0] : int*@  =>
+    (y[1] y[0])
+:]
+
+
+
+-----
+
+-- Widening
+#eval infer_reduce [:
+  λ y[0] : α[1] -> (α[1] -> (α[1] × α[1])) => 
+    (OUTPUT ; (y[0] hello;()))
+:]
+
+-- Widening
+#eval infer_reduce [:
+  λ y[0] : α[1] -> (α[1] -> (α[1] × α[1])) => 
+    (OUTPUT ; ((y[0] hello;()) world;()))
+:]
+
+
+-- Widening
+#eval infer_reduce [:
+  λ y[0] : α[1] -> (α[1] -> (α[1] × α[1])) => 
+  λ y[0] : hello*@ =>
+  λ y[0] : world*@ =>
+    OUTPUT ; ((y[2] y[1]) y[0])
+:]
+
+-- Widening
+#eval infer_reduce [:
+  λ y[0] : ∀ 1 => β[0] -> β[0] -> (β[0] × β[0]) => 
+  λ y[0] : hello*@ =>
+  λ y[0] : world*@ =>
+    OUTPUT ; ((y[2] y[1]) y[0])
+:]
+
+#eval infer_reduce [:
+  λ y[0] : α[1] -> (α[1] -> (α[1] × α[1])) => 
+  let y[0] = ((y[0] hello;()) world;()) =>
+    OUTPUT ; y[0]
+:]
+
+
+#eval infer_reduce [:
+  λ y[0] : ∀ 1 => β[0] -> β[0] -> (β[0] × β[0]) => 
+  λ y[0] : int*@  =>
+  λ y[0] : str*@  =>
+  let y[0] = ((y[2] y[1]) y[0]) =>
+  OUTPUT ; y[0]
+:]
+
+#eval infer_reduce [:
+  let y[0] = (hello ; ()) =>
+  y[0]
+:]
+
+-- Narrowing
+
+#eval [:
+  λ y[0] : uno*@ -> @ => y[0]
+:]
+#eval [:
+  λ y[0] : uno*@ -> @ => 
+  λ y[0] : dos*@ -> @ =>
+  λ y[0] =>
+    ((y[2] y[0]), (y[1] y[0]))
+:]
+#eval infer_reduce [:
+  λ y[0] : uno*@ -> @ => 
+  λ y[0] : dos*@ -> @ =>
+  OUTPUT ; (
+    λ y[0] => ((y[2] y[0]), (y[1] y[0]))
+  )
+:]
+#eval infer_reduce [:
+  λ y[0] : uno*@ -> @ => 
+  λ y[0] : dos*@ -> @ =>
+  OUTPUT ; (λ y[0] =>
+    ((y[2] y[0]), (y[1] y[0]))
+  )
+:]
+
+-- let-polymorphism: how generic?
+
+-- not generic
+#eval infer_reduce [:
+  ((λ y[0] : ⟨nat_⟩ => y[0]) zero;())
+:]
+
+-- not generic
+#eval infer_reduce [:
+  let y[0] = (λ y[0] : ⟨nat_⟩ => y[0]) =>
+  (y[0] zero;())
+:]
+
+-- not generic
+#eval infer_reduce [:
+  let y[0] = (λ y[0] : ⟨nat_⟩ => y[0]) =>
+  y[0]
+:]
+
+-- expected: ⊥ 
+#eval infer_reduce [:
+  let y[0] : (∀ 1 :: β[0] ≤ ⟨nat_⟩ => β[0] -> β[0]) = (λ y[0] : ⟨nat_⟩ => y[0]) =>
+  y[0]
+:]
+
+-- expected: true 
+#eval unify_test 
+[: (∀ 1 :: β[0] ≤ ⟨nat_⟩ => β[0] -> β[0]) :]
+[: ⟨nat_⟩ -> ⟨nat_⟩ :]
+
+-- expected: false 
+#eval unify_test 
+[: ⟨nat_⟩ -> ⟨nat_⟩ :]
+[: (∀ 1 :: β[0] ≤ ⟨nat_⟩ => β[0] -> β[0]) :]
+
+
+#eval infer_reduce [:
+  let y[0] : (∀ 1 :: ⟨nat_⟩ ≤ β[0] => β[0] -> β[0]) = (λ y[0] : ⟨nat_⟩ => y[0]) =>
+  y[0]
+:]
+
+-- generic enough
+-- but too redundant
+#eval infer_reduce [:
+  let y[0] : (∀ 1 :: β[0] ≤ ⟨nat_⟩ => β[0] -> β[0]) = (λ y[0] => y[0]) =>
+  (y[0] zero;())
+:]
+
+
+
+#eval infer_reduce [:
+  let y[0] = (λ y[0] => y[0]) =>
+  (y[0] zero;())
+:]
+
+#eval infer_reduce [:
+  let y[0] = (λ y[0] => y[0]) =>
+  y[0]
+:]
+
+#eval infer_reduce [:
+  let y[0] = (λ y[0] : ⟨nat_⟩ => ()) =>
+  let y[0] = (λ y[0] => ((y[1] y[0]), y[0])) =>
+  (y[0] zero;())
+:]
+
+-- let-polymorphism
+
+#eval infer_reduce [:
+  let y[0] = (λ y[0] : str*@ => hello ; y[0]) =>
+  (y[0] str;())
+:]
+
+#eval infer_reduce [:
+  let y[0] = (λ y[0] => hello ; y[0]) =>
+  (
+    y[0]
+  )
+:]
+
+#eval infer_reduce [:
+  let y[0] = (λ y[0] => hello ; y[0]) =>
+  (y[0] uno;())
+:]
+
+
+#eval infer_reduce [:
+  let y[0] = (λ y[0] => hello ; y[0]) =>
+  (
+    (y[0] uno;()),
+    (y[0] dos;())
+  )
+:]
+
+
+
+
+def repli := [:
+  ∀ 1 => β[0] -> (ν β[0] =>
+    (zero*@ -> nil*@) ∧
+    (∀ 2 :: β[2] ≤ (β[0] -> β[1]) =>
+      succ*β[0] -> cons*(β[3] × β[1])
     )
   )
+:]
 
-theorem not_lt_zero (n : Nat) : ¬ n < 0 :=
-  (fun h =>
-    let h : n + 1 ≤ 0 := h 
-    match n with
-      | 0 =>
-        let z := Nat.ne_of_lt h
-        absurd rfl z
-      | n' + 1 => 
-        let IH := not_lt_zero n'
-        let z : n' + 1 ≤ 0 := Nat.lt_of_succ_lt h 
-        (IH z)
+
+-----
+
+#eval unify_test 
+[: uno ~ @ ∧ dos ~ @ ∧ tres ~ @:]
+[: uno ~ @ ∧ tres ~ @:]
+
+#eval unify_test 
+[: uno ~ @ ∧ dos ~ @ ∧ tres ~ @:]
+[: ∀ 1 :: β[0] ≤ uno ~ @ ∨ dos ~ @ ∨ tres ~ @ => β[0]:]
+
+#eval unify_test 
+[: ∀ 1 :: β[0] ≤ uno ~ @ ∨ dos ~ @ ∨ tres ~ @ => β[0]:]
+[: uno ~ @ ∧ dos ~ @ ∧ tres ~ @:]
+
+
+#eval unify_test 
+[: uno ~ @ ∨ dos ~ @ ∨ tres ~ @ :]
+[:dos ~ @ ∧ tres ~ @ :]
+
+#eval unify_test 
+[:dos ~ @ ∧ tres ~ @ ∧ four ~ @:]
+[: uno ~ @ ∨ dos ~ @ ∨ tres ~ @ :]
+
+#eval unify_test 
+[: ∀ 1 :: β[0] ≤ uno ~ @ ∨ dos ~ @ ∨ tres ~ @ => β[0]:]
+[:dos ~ @ ∧ tres ~ @ ∧ four ~ @:]
+
+#eval unify_test 
+[: ∀ 1 :: uno ~ @ ∧ dos ~ @ ∧ tres ~ @ ≤ β[0] => β[0]:]
+[:dos ~ @ ∧ tres ~ @ :]
+
+#eval unify_test 
+[: ∀ 1 :: uno ~ @ ∧ dos ~ @ ∧ tres ~ @ ≤ β[0] => β[0]:]
+[: ∀ 1 :: uno ~ @ ∧ dos ~ @ ≤ β[0] => β[0]:]
+
+#eval unify_test 
+[: ∀ 1 :: uno ~ @ ∧ dos ~ @ ≤ β[0] => β[0]:]
+[: ∀ 1 :: uno ~ @ ∧ dos ~ @ ∧ tres ~ @ ≤ β[0] => β[0]:]
+
+#eval unify_test 
+[: ∀ 1 :: β[0] ≤ ⟨even⟩ => hello * β[0] :]
+[: ∀ 1 :: β[0] ≤ ⟨nat_⟩ => hello * β[0] :]
+
+#eval unify_test 
+[: ∀ 1 :: β[0] ≤ ⟨nat_⟩ => hello * β[0] :]
+[: ∀ 1 :: β[0] ≤ ⟨even⟩ => hello * β[0] :]
+
+#eval unify_test 
+[: ∀ 1 :: uno ~ @ ∧ dos ~ @ ∧ tres ~ @ ≤ β[0] => β[0]:]
+[: ∀ 1 :: uno ~ @ ∧ dos ~ @ ∧ four ~ @ ≤ β[0] => β[0]:]
+
+#eval unify_test 
+[: ∀ 1 :: β[0] ≤ uno ~ @ => β[0]:]
+[:uno ~ @ ∧ four ~ @:]
+
+#eval unify_test 
+[: ∀ 1 :: uno ~ @ ≤ β[0] => β[0]:]
+[:uno ~ @ ∧ four ~ @:]
+
+
+----- 
+
+def nat_to_unit := [: 
+  ν β[0] => 
+    (zero*@ -> @) ∧ 
+    (∀ 1 :: β[1] ≤ β[0] -> @ => 
+      (succ*β[0]) -> @) 
+:]
+
+def even_to_unit := [: 
+  ν β[0] => 
+    (zero*@ -> @) ∧ 
+    (∀ 1 :: β[1] ≤ β[0] -> @ => 
+      (succ*succ*β[0]) -> @)
+:]
+
+#eval unify_test 
+nat_to_unit
+[: (zero*@ -> @) :]
+
+#eval unify_test 
+nat_to_unit
+nat_to_unit
+
+#eval unify_test 
+nat_to_unit
+[: (succ*zero*@ -> @) :]
+
+#eval unify_test 
+even_to_unit
+[: (succ*succ*zero*@ -> @) :]
+
+#eval unify_test 
+even_to_unit
+[: (succ*zero*@ -> @) :]
+
+-- -- TODO: why does this diverge?
+-- #eval unify 3 {} Ty.top 
+-- [: 
+--     (zero*@ -> @) ∧ 
+--     (∀ 1 :: ⟨nat_to_unit⟩ ≤ β[0] -> @ => 
+--       (succ*β[0]) -> @) 
+-- :]
+-- [: 
+--     (zero*@ -> @) ∧ 
+--     (∀ 1 :: ⟨nat_to_unit⟩ ≤ β[0] -> @ => 
+--       (succ*succ*β[0]) -> @)
+-- :]
+
+-- #eval unify 3 {} Ty.top 
+-- nat_to_unit
+-- even_to_unit
+
+-- #eval unify 3 {} Ty.top 
+-- even_to_unit
+-- nat_to_unit
+
+-- #eval unify 3 {} Ty.top 
+-- nat_
+-- even
+
+#eval repli
+
+#eval [:
+  λ y[0] => fix (λ y[0] => λ[
+  for zero;() => nil;(),
+  for succ;y[0] => cons;(y[2], (y[1] y[0])) 
+  ]) 
+:]
+
+
+#eval infer_reduce [:
+  λ[
+  for zero;() => nil;(),
+  for succ;y[0] => cons;((), ()) 
+  ] 
+:]
+
+
+#eval [: (zero*@ -> nil*@) ∧ (succ*⊤ -> cons*(@ × ⊥)) :]
+
+#eval unify_reduce
+[: α[2] -> ((zero*@ -> nil*@) ∧ (succ*⊤ -> cons*(@ × @))) :]
+[: α[0] -> α[0] :]
+[: α[0] :]
+
+#eval infer_reduce_wt 
+[:
+  (λ y[0] => λ[
+  for zero;() => nil;(),
+  for succ;y[0] => cons;((), (y[1] y[0])) 
+  ]) 
+:]
+[: α[20] -> α[20] :]
+
+
+#eval [:
+  ∀ 1 => β[0] -> (ν β[0] =>
+    (zero*@ -> nil*@) ∧
+    (∀ 2 :: β[2] ≤ (β[0] -> β[1]) =>
+      succ*β[0] -> cons*(β[3] × β[1])
+    )
   )
+:]
+
+#eval unify_reduce
+[: (α[0] -> α[1]) -> ((zero*@ -> nil*@) ∧ (succ*α[0] -> cons*(@ × α[1]))) :]
+[: α[20] -> α[20] :]
+[: α[20] :]
+
+
+#eval infer_reduce [:
+  fix (λ y[0] => λ[
+  for zero;() => nil;(),
+  for succ;y[0] => cons;((), (y[1] y[0])) 
+  ]) 
+:]
+
+#eval infer_reduce_wt [:
+  fix (λ y[0] => λ[
+  for zero;() => nil;(),
+  for succ;y[0] => cons;((), (y[1] y[0])) 
+  ]) 
+:]
+[:
+  (zero*@ -> nil*@)
+:]
+
+
+#eval infer_reduce_wt [:
+  (λ y[0] => λ[
+  for zero;() => nil;(),
+  for succ;y[0] => cons;((), (y[1] y[0])) 
+  ]) 
+:]
+[:
+  (zero*@ -> nil*@)
+  ->
+  (zero*@ -> nil*@)
+:]
+
+#eval infer_reduce_wt [:
+  fix (λ y[0] => λ[
+  for zero;() => nil;(),
+  for succ;y[0] => cons;((), (y[1] y[0])) 
+  ]) 
+:]
+[:
+  ν β[0] => 
+  (∀ 2 :: β[2] ≤ (β[0] -> β[1]) => 
+    (zero*@ -> nil*@) ∧ 
+    (succ*β[0] -> cons*(@ × β[1]))
+  )
+:]
+
+
+#eval infer_reduce_wt [:
+  fix (λ y[0] => λ[
+  for zero;() => nil;(),
+  for succ;y[0] => cons;((), (y[1] y[0])) 
+  ]) 
+:]
+[:
+  ν β[0] => 
+  (
+    (zero*@ -> nil*@) ∧ 
+    (∀ 2 :: β[2] ≤ (β[0] -> β[1]) => 
+      (succ*β[0] -> cons*(@ × β[1]))
+    )
+  )
+:]
+
+
+#eval infer_reduce
+[:
+  λ y[0] : (ν β[0] => 
+    (
+      (zero*@ -> nil*@)
+    )
+  ) => (y[0] (zero;()))
+:]
+
+
+#eval infer_reduce
+[:
+  λ y[0] : (ν β[0] => 
+    (
+      (zero*@ -> nil*@) ∧ 
+      (∀ 2 :: β[2] ≤ (β[0] -> β[1]) => 
+        (succ*β[0] -> cons*(@ × β[1]))
+      )
+    )
+  ) => (y[0] (succ;zero;()))
+:]
+
+#eval infer_reduce
+[:
+  λ y[0] : (ν β[0] => 
+    (
+      (zero*@ -> nil*@) ∧ 
+      (∀ 2 :: β[2] ≤ (β[0] -> β[1]) => 
+        (succ*β[0] -> cons*(@ × β[1]))
+      )
+    )
+  ) => (y[0] (succ;_))
+:]
+
+#eval infer_reduce
+[:
+  λ y[0] : (ν β[0] => 
+    (
+      (zero*@ -> nil*@) ∧ 
+      (∀ 2 :: β[2] ≤ (β[0] -> β[1]) => 
+        (succ*β[0] -> cons*(@ × β[1]))
+      )
+    )
+  ) => (y[0] (succ;succ;_))
+:]
+
+#eval infer_reduce [:
+  λ y[0] : (
+    ν β[0] => ∀ 2 :: β[2] ≤ (β[1] -> β[0]) =>
+    ((zero*@ -> nil*@) ∧ (succ*β[1] -> cons*(@ × β[0])))
+  ) => (y[0] (succ;_))
+:]
+
+#eval infer_reduce [:
+  λ y[0] : (
+    ν β[0] => ∀ 2 :: β[2] ≤ (β[1] -> β[0]) =>
+    ((zero*@ -> nil*@) ∧ (succ*β[1] -> cons*(@ × β[0])))
+  ) => (y[0] (succ;succ;_))
+:]
+
+#eval infer_reduce [:
+  λ y[0] : (
+    ∀ 0 :: ⊥ ≤ ⊤ => (
+      ν β[0] => ∀ 2 :: β[2] ≤ (β[1] -> β[0]) =>
+      ((zero*@ -> nil*@) ∧ (succ*β[1] -> cons*(@ × β[0])))
+    )
+  ) => (y[0] (zero;()))
+:]
+
+---------
+
+#eval infer_reduce [:
+  let y[0] : (
+    ν β[0] => ∀ 2 :: β[2] ≤ (β[1] -> β[0]) =>
+    ((zero*@ -> nil*@) ∧ (succ*β[1] -> cons*(@ × β[0])))
+  ) = _ => (y[0] (zero;()))
+:]
+
+#eval infer_reduce [:
+  let y[0] : (
+    ν β[0] => ∀ 2 :: β[2] ≤ (β[1] -> β[0]) =>
+    ((zero*@ -> nil*@) ∧ (succ*β[1] -> cons*(@ × β[0])))
+  ) = _ => (y[0] (succ;succ;zero;()))
+:]
+
+#eval infer_reduce [:
+  let y[0] : (
+    ν β[0] => ∀ 2 :: β[2] ≤ (β[1] -> β[0]) =>
+    ((zero*@ -> nil*@) ∧ (succ*β[1] -> cons*(@ × β[0])))
+  ) = _ => (y[0] (succ;succ;_))
+:]
+
+#eval infer_reduce [:
+  let y[0] : (
+    ν β[0] => ∀ 2 :: β[2] ≤ (β[1] -> β[0]) =>
+    ((zero*@ -> nil*@) ∧ (succ*β[1] -> cons*(@ × β[0])))
+  ) = _ => y[0]
+:]
+
+
+#eval infer_reduce [:
+  let y[0] : (
+    ν β[0] => ∀ 2 :: β[2] ≤ (β[1] -> β[0]) =>
+      ((zero*@ -> nil*@) ∧ ((succ*β[1] -> cons*(l ~ @ ∧ (r ~ β[0] ∧ ⊤))) ∧ ⊤))
+  ) = _ => (y[0] (succ;succ;zero;()))
+:]
+
+
+#eval unify_test 
+[:
+  ν β[0] => ∀ 2 :: β[2] ≤ (β[1] -> β[0]) =>
+    ((zero*@ -> nil*@) ∧ ((succ*β[1] -> cons*(l ~ @ ∧ (r ~ β[0] ∧ ⊤))) ∧ ⊤))
+:]
+[:
+  α[0] -> α[1]
+:]
+
+#eval unify_test 
+[:
+  ν β[0] => ∀ 2 :: β[2] ≤ (β[1] -> β[0]) =>
+    (zero*@ -> nil*@) ∧ ((succ*β[1] -> cons*(l ~ @ ∧ r ~ β[0])))
+:]
+[:
+  α[0] -> α[1]
+:]
+
+#eval infer_reduce [:
+  let y[0] = fix(λ y[0] => λ[
+  for zero;() => nil;(),
+  for succ;y[0] => cons;((), (y[1] y[0])) 
+  ]) => 
+  (y[0] succ;zero;())
+:]
+
+
+#eval infer_reduce [:
+  let y[0] = fix(λ y[0] => λ[
+  for zero;() => nil;(),
+  for succ;y[0] => cons;((), (y[1] y[0])) 
+  ]) => 
+  y[0]
+:]
+
+#eval infer_test [:
+  let y[0] = fix(λ y[0] => λ[
+  for zero;() => nil;(),
+  for succ;y[0] => cons;((), (y[1] y[0])) 
+  ]) => 
+  y[0]
+:]
+[: α[30] :]
+
+#eval infer_test [:
+  let y[0] : (
+    ν β[0] => ∀ 2 :: β[2] ≤ (β[1] -> β[0]) =>
+    ((zero*@ -> nil*@) ∧ (succ*β[1] -> cons*(@ × β[0])))
+  ) = _ => y[0]
+:]
+[: α[30] :]
+
+#eval infer_reduce [:
+  let y[0] = fix(λ y[0] => λ[
+  for zero;() => nil;(),
+  for succ;y[0] => cons;((), (y[1] y[0])) 
+  ]) => 
+  (y[0] (zero;()))
+:]
+
+
+-- TODO: why does this fail?
+#eval infer_reduce [:
+  let y[0] : ⟨nat_⟩ = _ =>
+  let y[0] = fix(λ y[0] => λ[
+  for zero;() => nil;(),
+  for succ;y[0] => cons;((), (y[1] y[0])) 
+  ]) => 
+  (y[0] y[1])
+:]
+
+#eval infer_reduce [:
+  let y[0] : ⟨nat_⟩ = _ =>
+  let y[0] = fix(λ y[0] => λ[
+  for zero;() => nil;(),
+  for succ;y[0] => cons;((), (y[1] y[0])) 
+  ]) => 
+  y[1]
+:]
+
+#eval (extract_premise 0 [: 
+    ∀ 2 :: β[2] ≤ (β[1] -> β[0]) =>
+    ((zero*@ -> nil*@) ∧ (succ*β[1] -> cons*(@ × β[0])))
+:])
+
+#eval unify_test
+nat_
+[:
+μ β[0] => ∃ 2 :: β[1] ≤ β[2] =>
+zero*@ ∨ 
+succ*β[1]
+:]
+
+
+-- TODO: figure out why this fails
+#eval infer_test [:
+  fix(λ y[0] => λ[
+  for zero;() => nil;(),
+  for succ;y[0] => cons;((), (y[1] y[0])) 
+  ]) 
+:] [:
+  ν β[0] => ∀ 2 :: β[2] ≤ (β[1] -> β[0]) =>
+  ((zero*@ -> nil*@) ∧ (succ*β[1] -> cons*(@ × β[0])))
+:]
+
+#eval unify_test [:
+  ν β[0] => ∀ 2 :: β[2] ≤ (β[1] -> β[0]) =>
+  ((zero*@ -> nil*@) ∧ (succ*β[1] -> cons*(@ × β[0])))
+:] [:
+  ν β[0] => ∀ 2 :: β[2] ≤ (β[1] -> β[0]) =>
+  ((zero*@ -> nil*@) ∧ (succ*β[1] -> cons*(@ × β[0])))
+:]
+
+-- TODO: why does this fail?
+#eval unify_test [:
+  ν β[0] => ∀ 2 :: β[2] ≤ (β[1] -> β[0]) =>
+  ((zero*@ -> nil*@) ∧ (succ*β[1] -> cons*(@ × β[0])))
+:] [:
+  ∀ 1 :: β[0] ≤ (⟨nat_⟩) =>
+    (β[0] -> (∃ 1 :: (β[1] × β[0]) ≤ ⟨nat_list⟩ => β[0]))
+:]
+
+#eval unify_test [:
+  ∀ 1 :: β[0] ≤ (⟨nat_⟩) =>
+    (β[0] -> (∃ 1 :: (β[1] × β[0]) ≤ ⟨nat_list⟩ => β[0]))
+:] [:
+  ν β[0] => ∀ 2 :: β[2] ≤ (β[1] -> β[0]) =>
+  ((zero*@ -> nil*@) ∧ (succ*β[1] -> cons*(@ × β[0])))
+:]
+
+
+-- TODO: figure out why this fails
+#eval infer_reduce_wt [:
+  (λ y[0] => λ[
+  for zero;() => nil;(),
+  for succ;y[0] => cons;((), (y[1] y[0])) 
+  ]) 
+:]
+[:
+  (ν β[0] => ∀ 2 :: β[2] ≤ (β[0] -> β[1]) =>
+    ((zero*@ -> nil*@) ∧ (succ*β[0] -> cons*(@ × β[1])))
+  )
+  ->
+  (ν β[0] => ∀ 2 :: β[2] ≤ (β[0] -> β[1]) =>
+    ((zero*@ -> nil*@) ∧ (succ*β[0] -> cons*(@ × β[1])))
+  )
+:]
+
+
+#eval infer_reduce [:
+  fix(λ y[0] => λ[
+  for zero;() => nil;(),
+  for succ;y[0] => cons;((), (y[1] y[0])) 
+  ]) 
+:]
+
+#eval infer_reduce [:
+  let y[0] = fix(λ y[0] => λ[
+  for zero;() => nil;(),
+  for succ;y[0] => cons;((), (y[1] y[0])) 
+  ]) => 
+  y[0]
+:]
+
+#eval unify_reduce 
+[:
+  (ν β[0] => 
+    (
+      (zero*@ -> nil*@) ∧ 
+      (∀ 2 :: β[2] ≤ (β[0] -> β[1]) => 
+        (succ*β[0] -> cons*(@ × β[1]))
+      )
+    )
+  )
+:]
+[:
+  α[0] -> α[1]
+:]
+[: α[0] :]
+
+
+
+#eval extract_premise 0 [:
+    (
+      (zero*@ -> nil*@) ∧ 
+      (∀ 2 :: β[2] ≤ (β[0] -> β[1]) => 
+        (succ*β[0] -> cons*(@ × β[1]))
+      )
+    )
+:]
+
+#eval rewrite_function_type [:
+  ν β[0] =>
+    (
+      (zero*@ -> nil*@) ∧ 
+      (∀ 2 :: β[2] ≤ (β[0] -> β[1]) => 
+        (succ*β[0] -> cons*(@ × β[1]))
+      )
+    )
+:]
+
+
+#eval unify_reduce
+[:
+  (∀ 1 :: β[0] ≤ (μ β[0] => zero*@ ∨ (∃ 2 :: β[0] ≤ β[2] => succ*β[0])) =>
+    (β[0] ->
+      (∃ 1 :: 
+        (β[1] × β[0]) ≤ (μ β[0] => 
+          (zero*@ × nil*@) ∨
+          (∃ 2 :: (β[0] × β[1]) ≤ β[2] => (succ*β[0] × cons*(@ × β[1])))
+        ) =>
+        β[0]
+      )
+    )
+  )
+:]
+[: α[0] -> α[1] :]
+[: α[1] :]
+
+-- false: why does this fail?
+-- ∀ can't be instantiated 
+-- safe to fail, but not lenient
+#eval unify_test [:
+  ν β[0] => ∀ 2 :: β[2] ≤ (β[1] -> β[0]) =>
+  ((zero*@ -> nil*@) ∧ (succ*β[1] -> cons*(@ × β[0])))
+:] [:
+  ∀ 1 :: β[0] ≤ (⟨nat_⟩) =>
+    (β[0] -> (∃ 1 :: (β[1] × β[0]) ≤ ⟨nat_list⟩ => β[0]))
+:]
+
+-- false: why does this fail?
+-- ν can't be unrolled
+-- safe to fail, but not lenient
+#eval unify_test 
+[:
+  ∀ 1 :: β[0] ≤ (⟨nat_⟩) =>
+    (β[0] -> (∃ 1 :: (β[1] × β[0]) ≤ ⟨nat_list⟩ => β[0]))
+:]
+[:
+  ν β[0] => ∀ 2 :: β[2] ≤ (β[1] -> β[0]) =>
+  ((zero*@ -> nil*@) ∧ (succ*β[1] -> cons*(@ × β[0])))
+:] 
+
+#eval unify_test [:
+  (∀ 1 :: β[0] ≤ (μ β[0] => zero*@ ∨ (∃ 2 :: β[0] ≤ β[2] => succ*β[0])) =>
+    (β[0] ->
+      (∃ 1 :: 
+        (β[1] × β[0]) ≤ (μ β[0] => 
+          (zero*@ × nil*@) ∨
+          (∃ 2 :: (β[0] × β[1]) ≤ β[2] => (succ*β[0] × cons*(@ × β[1])))
+        ) =>
+        β[0]
+      )
+    )
+  )
+:] [:
+  (∀ 1 :: β[0] ≤ (μ β[0] => zero*@ ∨ (∃ 2 :: β[0] ≤ β[2] => succ*β[0])) =>
+    (β[0] ->
+      (∃ 1 :: 
+        (β[1] × β[0]) ≤ (μ β[0] => 
+          (zero*@ × nil*@) ∨
+          (∃ 2 :: (β[0] × β[1]) ≤ β[2] => (succ*β[0] × cons*(@ × β[1])))
+        ) =>
+        β[0]
+      )
+    )
+  )
+:]
+
+-- TODO: why does this fail?
+#eval unify_test [:
+  (∀ 1 :: β[0] ≤ ⟨nat_⟩ =>
+    (β[0] ->
+      (∃ 1 :: 
+        (β[1] × β[0]) ≤ ⟨nat_list⟩ =>
+        β[0]
+      )
+    )
+  )
+:] [:
+  (∀ 1 :: β[0] ≤ ⟨nat_⟩ =>
+    (β[0] ->
+      (∃ 1 :: 
+        (β[1] × β[0]) ≤ ⟨nat_list⟩ =>
+        β[0]
+      )
+    )
+  )
+:]
+
+#eval unify_test even nat_
+
+#eval unify_test [:
+  ⟨nat_⟩ -> @
+:] [:
+  ⟨even⟩ -> @ 
+:]
+
+-- expected: true
+#eval unify_test [:
+  (∀ 1 :: β[0] ≤ ⟨nat_⟩ =>
+    (β[0] -> @)
+  )
+:] [:
+  (∀ 1 :: β[0] ≤ ⟨even⟩ =>
+    (β[0] -> @)
+  )
+:]
+
+-- expected: false 
+#eval unify_test [:
+  (∀ 1 :: β[0] ≤ ⟨even⟩ =>
+    (β[0] -> @)
+  )
+:] [:
+  (∀ 1 :: β[0] ≤ ⟨nat_⟩ =>
+    (β[0] -> @)
+  )
+:]
+
+-- expected: true
+#eval unify_test [:
+  (∀ 1 :: β[0] ≤ ⟨nat_⟩ =>
+    (β[0])
+  )
+:] [:
+  (∀ 1 :: β[0] ≤ ⟨even⟩ =>
+    (β[0])
+  )
+:]
+
+-- expected: false 
+-- this is overly strict, but safe 
+-- there is no way for the LHS to know to instantiate with ⊥ vs nat_
+#eval unify_test [:
+  (∀ 1 :: β[0] ≤ ⟨even⟩ =>
+    (β[0])
+  )
+:] [:
+  (∀ 1 :: β[0] ≤ ⟨nat_⟩ =>
+    (β[0])
+  )
+:]
+
+-- expected: true 
+#eval unify_test [:
+  (∀ 1 :: ⟨even⟩ ≤ β[0] =>
+    (β[0])
+  )
+:] [:
+  (∀ 1 :: ⟨nat_⟩ ≤ β[0] =>
+    (β[0])
+  )
+:]
+
+
+-- expected: false 
+-- RHS could be ⊥, but LHS must be > ⊥
+#eval unify_test [:
+  (∀ 1 :: ⟨even⟩ ≤ β[0] =>
+    (β[0])
+  )
+:] [:
+  (∀ 1 => (β[0]))
+:]
+
+#eval unify_test even [: ⊥ :]
+
+-- expected: false 
+-- RHS could be ⊤ -> @, but LHS must be > even -> @ 
+-- must give negative positions ⊤, and positive positions ⊥
+-- bound flips based on negative/positive position
+#eval unify_test [:
+  (∀ 1 :: β[0] ≤ ⟨even⟩ =>
+    (β[0] -> @)
+  )
+:] [:
+  (∀ 1 => (β[0] -> @))
+:]
+
+-- expected: true 
+#eval unify_test [:
+  (∀ 1 :: β[0] ≤ ⟨nat_⟩ =>
+    (β[0] -> @)
+  )
+:] [:
+  (∀ 1 :: β[0] ≤ ⟨even⟩ =>
+    (β[0] -> @)
+  )
+:]
+
+-- expected: false
+#eval unify_test [:
+  (∀ 1 :: β[0] ≤ ⟨even⟩ =>
+    (β[0] -> @)
+  )
+:] [:
+  (∀ 1 :: β[0] ≤ ⟨nat_⟩ =>
+    (β[0] -> @)
+  )
+:]
+
+-- expected: true 
+#eval unify_test [:
+  (∃ 1 :: β[0] ≤ ⟨even⟩ =>
+    (β[0])
+  )
+:] [:
+  (∃ 1 :: β[0] ≤ ⟨nat_⟩ =>
+    (β[0])
+  )
+:]
+
+-- expected: false 
+#eval unify_test [:
+  (∃ 2 :: β[0] × β[1] ≤ ⟨nat_⟩ × ⟨nat_⟩ =>
+    β[0] × β[1]
+  )
+:] [:
+  (∃ 1 :: β[0] ≤ ⟨nat_⟩ =>
+    (succ*@ × β[0])
+  )
+:]
+
+-- expected: true 
+#eval unify_test [:
+  (∃ 1 :: β[0] ≤ ⟨even⟩ =>
+    (β[0])
+  )
+:] nat_
+#eval unify_test [:
+  (∃ 1 =>
+    (β[0])
+  )
+:] nat_
+
+-- expected: false 
+#eval unify_test [:
+  (∃ 1 :: β[0] ≤ ⟨nat_⟩ =>
+    (β[0])
+  )
+:] [:
+  (∃ 1 :: β[0] ≤ ⟨even⟩ =>
+    (β[0])
+  )
+:]
+
+
+-- expected: false
+-- β[0] could be TOP
+#eval unify_test [:
+  (∃ 1 :: ⟨even⟩ ≤ β[0] =>
+    (β[0])
+  )
+:] [:
+  (∃ 1 :: β[0] ≤ ⟨even⟩ =>
+    (β[0])
+  )
+:]
+
+#eval unify_test [:
+  ⊤ 
+:] [:
+  (∃ 1 :: β[0] ≤ ⟨even⟩ =>
+    (β[0])
+  )
+:]
+
+
+
+
+/-
+first order quantification
+
+μ NL .
+  {(0, [])} ∨ 
+  ∃ (n, l) : NL . 
+    (n + 1,  () :: l)  
+
+ν N2L .
+  {0 => []} ∧ 
+  ∀ n -> l : N2L .  WRONG
+    {n + 1 => () :: l }
+
+ν N2L .
+  0 -> nil*unit ∧ 
+  ∀ N2L ≤ N -> L .    
+    N + 1 => unit :: L
+
+--- 
+by second order quantification with subtyping rather than first order with membership,
+we avoid mapping between terms and types in unification procedure.
+We also enable the succient corecursive definitions of functions.
+
+-/
+
+/-
+translating Liquid types into relational types
+
+List with len where
+[] : {v ∈ List | len v = 0} | 
+() :: (xs : List) : {v ∈ List | len v = (len xs) + 1} | 
+
+n : Nat -> {v ∈ List | len v = n}
+
+...
+
+∀ N . N ≤ Nat => N -> (∃ L . 
+  (N × L) ≤ (μ N' × L' .  (0 × []) | (N' + 1 × () :: L'))  =>
+  L
+)
+
+...
+
+ν N -> L .
+  0 -> [] ∧ 
+  N + 1 -> () :: L  
+-/
