Main.lean
@@ -1,0 +1,4 @@
+import Theory
+
+def main : IO Unit :=
+  IO.println s!"Hello, {hello}!"
