Practice.lean
@@ -1,0 +1,144 @@
+import Mathlib.Tactic.Basic
+import Mathlib.Tactic.LeftRight
+
+
+lemma v1 (P Q R : Prop) : P ∧ (Q ∨ R) ↔ (P ∧ Q) ∨ (P ∧ R) := by
+(constructor;
+  (intro h;
+    cases h with 
+      | intro hP hQR =>
+        cases hQR with
+          | inl hQ => 
+            left; constructor;
+              assumption;
+              assumption
+          | inr hR => 
+            right; constructor;
+                assumption;
+              assumption
+  );
+  (intro h;
+    cases h with
+      | inl hPQ => 
+        cases hPQ with 
+          | intro hP hQ => 
+            constructor;
+              assumption;
+              left; assumption
+      | inr hPR =>
+        cases hPR with
+          | intro hP hR =>
+            constructor;
+              assumption;
+              right; assumption
+  )
+)
+
+lemma v2 (P Q R : Prop) : P ∧ (Q ∨ R) ↔ (P ∧ Q) ∨ (P ∧ R) := 
+  ((Iff.intro
+    ((λ h : P ∧ (Q ∨ R) =>
+      (match h with
+        | And.intro hP hQR => (match hQR with
+            | Or.inl hQ => Or.inl (And.intro hP hQ : P ∧ Q)
+            | Or.inr hR => Or.inr (And.intro hP hR : P ∧ R)
+        )
+      )
+    ) : P ∧ (Q ∨ R) -> (P ∧ Q) ∨ (P ∧ R))
+    ((λ h : P ∧ Q ∨ P ∧ R =>
+      (And.intro 
+        ((match h with
+          | Or.inl (And.intro hP hQ) => hP
+          | Or.inr (And.intro hP hR) => hP
+        ) : P)
+        ((match h with
+          | Or.inl (And.intro hP hQ) => Or.inl hQ 
+          | Or.inr (And.intro hP hR) => Or.inr hR
+        ) : Q ∨ R)
+      )
+    ) : (P ∧ Q) ∨ (P ∧ R) -> P ∧ (Q ∨ R))
+  ) : P ∧ (Q ∨ R) ↔ (P ∧ Q) ∨ (P ∧ R))
+
+class MyAdd (a : Type) where
+  add : a -> a -> a
+
+#check @MyAdd.add
+
+instance : MyAdd Nat where
+  add := Nat.add
+
+instance : MyAdd Int where
+  add := Int.add
+
+instance : MyAdd Float where
+  add := Float.add
+
+def double [inst : Add a] (x : a) : a :=
+  inst.add x x
+
+#check @double
+-- @double : {a : Type} → [inst : Add a] → a → a
+
+-- #eval double 10
+-- 20
+
+
+
+#check Nat.ne_of_lt
+
+example : ¬ 0 < 0 :=
+  ((fun h => 
+    let x := (Nat.ne_of_lt h)
+    let y := (absurd rfl x)
+    y
+  ) : ¬ 0 < 0)
+
+#check @absurd
+example (n : Nat) (h : n ≠ 0) : .succ (.pred n) = n := 
+  ((match n with
+    | Nat.zero => absurd rfl h
+    | Nat.succ m => rfl 
+  ) : .succ (.pred n) = n)
+
+example (n : Nat) (h : n ≠ 0) : .succ (.pred n) = n := by
+  cases n with
+  | zero =>
+    -- goal: h : 0 ≠ 0 ⊢ succ (pred 0) = 0
+    apply absurd rfl h
+  | succ m =>
+    -- second goal: h : succ m ≠ 0 ⊢ succ (pred (succ m)) = succ m
+    rfl
+
+
+-- induction with term and tactics
+def add : Nat → Nat → Nat
+  | m, .zero   => m
+  | m, .succ n => .succ (add m n)
+
+theorem add_zero (m : Nat)   : add m .zero = m := rfl
+theorem add_succ (m n : Nat) : add m (.succ n) = .succ (add m n) := rfl
+
+theorem zero_add : ∀ n, add .zero n = n
+  | .zero   => rfl
+  | .succ n => congrArg Nat.succ (zero_add n)
+
+#check @congrArg
+example : ∀ n, add .zero n = n := by
+  (intro n;
+    (induction n with
+      | zero => apply rfl 
+      | succ n IH => apply congrArg Nat.succ IH
+    )
+  )
+
+theorem not_lt_zero (n : Nat) : ¬ n < 0 :=
+  (fun h =>
+    let h : n + 1 ≤ 0 := h 
+    match n with
+      | 0 =>
+        let z := Nat.ne_of_lt h
+        absurd rfl z
+      | n' + 1 => 
+        let IH := not_lt_zero n'
+        let z : n' + 1 ≤ 0 := Nat.lt_of_succ_lt h 
+        (IH z)
+  )
