lakefile.lean
@@ -1,14 +1,27 @@
 import Lake
 open Lake DSL
 
-package test {
+-- ll -> ≪
+-- gg -> ≫
+
+package slim {
   -- add any package configuration options here
 }
 
 require mathlib from git
   "https://github.com/leanprover-community/mathlib4.git"
 
-@[defaultTarget]
-lean_lib Test {
+-- @[default_target]
+-- lean_lib Practice {
+--   -- add any library configuration options here
+-- }
+
+@[default_target]
+lean_lib Theory {
   -- add any library configuration options here
+}
+
+@[default_target]
+lean_exe «greeting»  {
+  root := `Main
 }
